m

DynamoDbEncryption/dafny/StructuredEncryption/src/Paths.dfy
@@ -36,18 +36,18 @@ module StructuredEncryptionPaths {
     function method canonicalPath(table : GoodString)
       : (ret : CanonicalPath)
       ensures ret ==
-          //= specification/structured-encryption/header.md#canonical-path
-          //= type=implication
-          //# The canonical path MUST start with the UTF8 encoded table name.
-          UTF8.Encode(table).value
-          //= specification/structured-encryption/header.md#canonical-path
-          //= type=implication
-          //# This MUST be followed by the depth of the Terminal within Structured Data.
-        + UInt64ToSeq(|parts| as uint64)
-          //= specification/structured-encryption/header.md#canonical-path
-          //= type=implication
-          //# This MUST be followed by the encoding for each Structured Data in the path, including the Terminal itself.
-        + MakeCanonicalPath(parts)
+              //= specification/structured-encryption/header.md#canonical-path
+              //= type=implication
+              //# The canonical path MUST start with the UTF8 encoded table name.
+              UTF8.Encode(table).value
+              //= specification/structured-encryption/header.md#canonical-path
+              //= type=implication
+              //# This MUST be followed by the depth of the Terminal within Structured Data.
+              + UInt64ToSeq(|parts| as uint64)
+              //= specification/structured-encryption/header.md#canonical-path
+              //= type=implication
+              //# This MUST be followed by the encoding for each Structured Data in the path, including the Terminal itself.
+              + MakeCanonicalPath(parts)
     {
       var tableName := UTF8.Encode(table).value;
       var depth := UInt64ToSeq(|parts| as uint64);
@@ -76,7 +76,7 @@ module StructuredEncryptionPaths {
   {
     TerminalLocation([Map(attr)])
   }
-  
+
   function method {:opaque} SimpleCanon(table : GoodString, attr : GoodString)
     : CanonicalPath
   {
@@ -94,10 +94,12 @@ module StructuredEncryptionPaths {
     //# For Structured Data in Structured Data Maps, this MUST be a 0x24 byte ($ in UTF-8),
     //# followed by the length of the key, followed by the key as a UTF8 string.
     ensures s.Map? ==> ret == [MAP_TAG] + UInt64ToSeq(|s.key| as uint64) + UTF8.Encode(s.key).value
+    ensures s.Map? ==> |ret| == 9 + |UTF8.Encode(s.key).value|
     //= specification/structured-encryption/header.md#canonical-path
     //= type=implication
     //# For Structured Data in Structured Data Lists, this MUST be a 0x23 byte (# in UTF-8), followed by the numerical index.
     ensures s.List? ==> ret == [ARRAY_TAG] + UInt64ToSeq(s.pos as uint64)
+    ensures s.List? ==> |ret| == 9
   {
     match s {
       case Map(key) => [MAP_TAG] + UInt64ToSeq(|key| as uint64) + UTF8.Encode(key).value
@@ -107,7 +109,9 @@ module StructuredEncryptionPaths {
 
   // get the Canonical Path for these Selectors
   function method {:tailrecursion} MakeCanonicalPath(src : SelectorList)
-   : CanonicalPath
+    : (ret : CanonicalPath)
+    ensures |src| == 0 ==> ret == []
+    ensures |src| == 1 ==> ret == CanonicalPart(src[0])
   {
     if |src| == 0 then
       []
@@ -115,31 +119,197 @@ module StructuredEncryptionPaths {
       CanonicalPart(src[0]) + MakeCanonicalPath(src[1..])
   }
 
-// End code, begin lemmas. 
-// The only useful one is SimpleCanonUnique
-// The others are here to prove that
+  // End code, begin lemmas.
+  // The only useful ones are SimpleCanonUnique and FullPathUnique
+  // The others are here to prove those
+  // SimpleCanon and SimpleCanonUnique should be retired
 
-  lemma CanonicalPartMapUnique(x : Selector, y : Selector)
+
+  // x != y ==> x.canonicalPath != y.canonicalPath, so we can map with it
+  lemma FullPathUnique(table : GoodString)
+    ensures forall x : TerminalLocation, y : TerminalLocation
+              :: x != y ==> x.canonicalPath(table) != y.canonicalPath(table)
+  {
+    forall x : TerminalLocation, y : TerminalLocation
+      ensures x != y ==> x.canonicalPath(table) != y.canonicalPath(table) {
+      if x != y {
+        FullPathUnique2(table, x, y);
+      }
+    }
+  }
+
+  lemma FullPathUnique2(table : GoodString, x : TerminalLocation, y : TerminalLocation)
+    requires x != y
+    ensures x.canonicalPath(table) != y.canonicalPath(table)
+  {
+    PathUnique2(x.parts, y.parts);
+    var cpX := x.canonicalPath(table);
+    var cpY := y.canonicalPath(table);
+    var tableName := UTF8.Encode(table).value;
+    assert tableName < cpX;
+    assert tableName < cpY;
+    if |x.parts| == |y.parts| {
+      var prefix := tableName + UInt64ToSeq(|x.parts| as uint64);
+      assert cpX == prefix + MakeCanonicalPath(x.parts);
+      assert cpY == prefix + MakeCanonicalPath(y.parts);
+      PathUnique2(x.parts, y.parts);
+      OnePlusOne(prefix, MakeCanonicalPath(x.parts), MakeCanonicalPath(y.parts));
+      assert cpX != cpY;
+    } else {
+      assert UInt64ToSeq(|x.parts| as uint64) != UInt64ToSeq(|y.parts| as uint64);
+      assert (tableName + UInt64ToSeq(|x.parts| as uint64)) < cpX;
+      assert (tableName + UInt64ToSeq(|y.parts| as uint64)) < cpY;
+      OnePlusOne(tableName, UInt64ToSeq(|x.parts| as uint64), UInt64ToSeq(|y.parts| as uint64));
+      assert (tableName + UInt64ToSeq(|x.parts| as uint64)) != (tableName + UInt64ToSeq(|y.parts| as uint64));
+      assert cpX != cpY;
+    }
+  }
+
+  // x != y ==> MakeCanonicalPath(x) != MakeCanonicalPath(y), so we can map with it
+  lemma PathUnique()
+    ensures forall x : SelectorList, y : SelectorList
+              :: x != y ==> MakeCanonicalPath(x) != MakeCanonicalPath(y)
+  {
+    forall x : SelectorList, y : SelectorList
+      ensures x != y ==> MakeCanonicalPath(x) != MakeCanonicalPath(y) {
+      if x != y {
+        PathUnique2(x, y);
+      }
+    }
+  }
+
+  lemma PathUnique2(x : SelectorList, y : SelectorList)
+    requires x != y
+    ensures MakeCanonicalPath(x) != MakeCanonicalPath(y)
+  {
+    if |x| == 0 || |y| == 0 {
+
+    } else if x[0] != y[0] {
+      CanonicalPartMapUnique(x[0], y[0]);
+      assert CanonicalPart(x[0]) != CanonicalPart(y[0]);
+      SelectorNeverPrefix(x[0], y[0]);
+      assert CanonicalPart(x[0]) <= MakeCanonicalPath(x);
+      assert CanonicalPart(y[0]) <= MakeCanonicalPath(y);
+      assert MakeCanonicalPath(x) == CanonicalPart(x[0]) + MakeCanonicalPath(x[1..]);
+      assert MakeCanonicalPath(y) == CanonicalPart(y[0]) + MakeCanonicalPath(y[1..]);
+      assert MakeCanonicalPath(x) != MakeCanonicalPath(y);
+    } else {
+      assert(x[1..] != y[1..]);
+      PathUnique2(x[1..], y[1..]);
+      assert CanonicalPart(x[0]) == CanonicalPart(y[0]);
+      assert MakeCanonicalPath(x[1..]) != MakeCanonicalPath(y[1..]);
+      OnePlusOne(CanonicalPart(x[0]), MakeCanonicalPath(x[1..]), MakeCanonicalPath(y[1..]));
+      assert CanonicalPart(x[0]) + MakeCanonicalPath(x[1..]) != CanonicalPart(x[0]) + MakeCanonicalPath(y[1..]);
+      assert CanonicalPart(x[0]) + MakeCanonicalPath(x[1..]) != CanonicalPart(y[0]) + MakeCanonicalPath(y[1..]);
+      assert MakeCanonicalPath(x) != MakeCanonicalPath(y);
+    }
+  }
+
+lemma {:axiom} Utf8EncodeIsDistributive(x: string)
+    requires UTF8.Encode(x).Success?
+    ensures forall head, tail | head + tail == x
+      :: UTF8.Encode(head).Success?
+          ==>
+            && UTF8.Encode(tail).Success?
+            && UTF8.Encode(head).value + UTF8.Encode(tail).value == UTF8.Encode(x).value
+
+  // must be true for any correct UTF8 implementation
+  lemma /*{:axiom}*/ Utf8EncodeUnique(x : string, y : string)
+    requires UTF8.Encode(x).Success?
+    requires UTF8.Encode(y).Success?
+    // ensures x == y ==> UTF8.Encode(x).value == UTF8.Encode(y).value
+    // ensures x != y ==> UTF8.Encode(x).value != UTF8.Encode(y).value
+    // ensures x <= y ==> UTF8.Encode(x).value <= UTF8.Encode(y).value
+    // ensures x <  y ==> UTF8.Encode(x).value <  UTF8.Encode(y).value
+    // ensures y <= x ==> UTF8.Encode(y).value <= UTF8.Encode(x).value
+    // ensures y <  x ==> UTF8.Encode(y).value <  UTF8.Encode(x).value
+    ensures !(x <= y) ==> !(UTF8.Encode(x).value <= UTF8.Encode(y).value)
+    // ensures !(x <  y) ==> !(UTF8.Encode(x).value <  UTF8.Encode(y).value)
+    // ensures !(y <= x) ==> !(UTF8.Encode(y).value <= UTF8.Encode(x).value)
+    // ensures !(y <  x) ==> !(UTF8.Encode(y).value <  UTF8.Encode(x).value)
+  {
+    Utf8EncodeIsDistributive(x);
+    Utf8EncodeIsDistributive(y);
+  }
+
+  // // must be true for any correct UTF8 implementation
+  // lemma {:axiom} Utf8DecodeUnique(x : seq<uint8>, y : seq<uint8>)
+  //   requires UTF8.Decode(x).Success?
+  //   requires UTF8.Decode(y).Success?
+  //   ensures x == y ==> UTF8.Decode(x).value == UTF8.Decode(y).value
+  //   ensures x != y ==> UTF8.Decode(x).value != UTF8.Decode(y).value
+  //   ensures x <= y ==> UTF8.Decode(x).value <= UTF8.Decode(y).value
+  //   ensures x <  y ==> UTF8.Decode(x).value <  UTF8.Decode(y).value
+  //   ensures y <= x ==> UTF8.Decode(y).value <= UTF8.Decode(x).value
+  //   ensures y <  x ==> UTF8.Decode(y).value <  UTF8.Decode(x).value
+  //   ensures !(x <= y) ==> !(UTF8.Decode(x).value <= UTF8.Decode(y).value)
+  //   ensures !(x <  y) ==> !(UTF8.Decode(x).value <  UTF8.Decode(y).value)
+  //   ensures !(y <= x) ==> !(UTF8.Decode(y).value <= UTF8.Decode(x).value)
+  //   ensures !(y <  x) ==> !(UTF8.Decode(y).value <  UTF8.Decode(x).value)
+
+  lemma SelectorNeverPrefixMap(x : Selector, y : Selector)
+    requires x != y
     requires x.Map?
     requires y.Map?
+    ensures !(CanonicalPart(x) <= CanonicalPart(y))
+    ensures !(CanonicalPart(y) <= CanonicalPart(x))
+  {
+    if |x.key| != |y.key| {
+      assert CanonicalPart(x)[1..9] != CanonicalPart(y)[1..9];
+    } else {
+      assert |x.key| == |y.key|;
+      assert x.key != y.key;
+      assert !(x.key <= y.key);
+      assert !(y.key <= x.key);
+      Utf8EncodeUnique(x.key, y.key);
+      assert !(UTF8.Encode(x.key).value <= UTF8.Encode(y.key).value);
+      assert !(UTF8.Encode(y.key).value <= UTF8.Encode(x.key).value);
+      assert CanonicalPart(x) == [MAP_TAG] + UInt64ToSeq(|x.key| as uint64) + UTF8.Encode(x.key).value;
+      assert CanonicalPart(y) == [MAP_TAG] + UInt64ToSeq(|y.key| as uint64) + UTF8.Encode(y.key).value;
+      assert CanonicalPart(x)[0..9] == CanonicalPart(y)[0..9];
+    }
+  }
+
+  lemma SelectorNeverPrefixList(x : Selector, y : Selector)
+    requires x != y
+    requires x.List?
+    requires y.List?
+    ensures !(CanonicalPart(x) <= CanonicalPart(y))
+    ensures !(CanonicalPart(y) <= CanonicalPart(x))
+  {
+    assert x.pos != y.pos;
+    var cpX := CanonicalPart(x);
+    var cpY := CanonicalPart(y);
+    assert cpX == [ARRAY_TAG] + UInt64ToSeq(x.pos as uint64);
+    assert cpY == [ARRAY_TAG] + UInt64ToSeq(y.pos as uint64);
+    assert UInt64ToSeq(x.pos as uint64) != UInt64ToSeq(y.pos as uint64);
+    OnePlusOne([ARRAY_TAG], UInt64ToSeq(x.pos as uint64), UInt64ToSeq(y.pos as uint64));
+    assert cpX != cpY;
+    assert !(cpY <= cpX);
+    assert !(cpX <= cpY);
+  }
+
+  lemma SelectorNeverPrefix(x : Selector, y : Selector)
+    requires x != y
+    ensures !(CanonicalPart(x) <= CanonicalPart(y))
+    ensures !(CanonicalPart(y) <= CanonicalPart(x))
+  {
+    if x.Map? && y.Map? {
+      SelectorNeverPrefixMap(x, y);
+    } else if x.List? && y.List? {
+      SelectorNeverPrefixList(x, y);
+    } else {
+      assert CanonicalPart(x)[0] != CanonicalPart(y)[0];
+      assert !(CanonicalPart(x) <= CanonicalPart(y));
+      assert !(CanonicalPart(y) <= CanonicalPart(x));
+    }
+  }
+
+  lemma CanonicalPartMapUnique(x : Selector, y : Selector)
     requires x != y
     ensures CanonicalPart(x) != CanonicalPart(y)
   {
-    assert x.key != y.key;
-    assert CanonicalPart(x) == [MAP_TAG] + UInt64ToSeq(|x.key| as uint64) + UTF8.Encode(x.key).value;
-    assert CanonicalPart(y) == [MAP_TAG] + UInt64ToSeq(|y.key| as uint64) + UTF8.Encode(y.key).value;
-    assert UTF8.Encode(x.key).value != UTF8.Encode(y.key).value;
-    if |x.key| == |y.key| {
-      var prefix := [MAP_TAG] + UInt64ToSeq(|y.key| as uint64);
-      assert CanonicalPart(x) == prefix + UTF8.Encode(x.key).value;
-      assert CanonicalPart(y) == prefix + UTF8.Encode(y.key).value;
-      OnePlusOne(prefix, UTF8.Encode(x.key).value, UTF8.Encode(y.key).value);
-      assert CanonicalPart(x) != CanonicalPart(y);
-    } else {
-      assert UInt64ToSeq(|x.key| as uint64) != UInt64ToSeq(|y.key| as uint64);
-      assert CanonicalPart(x)[1..9] == UInt64ToSeq(|x.key| as uint64);
-      assert CanonicalPart(y)[1..9] == UInt64ToSeq(|y.key| as uint64);
-    }
+    SelectorNeverPrefix(x, y);
   }
 
   lemma OnePart(src : SelectorList)
@@ -168,20 +338,8 @@ module StructuredEncryptionPaths {
     requires x != y
     ensures SimpleCanon(table, x) != SimpleCanon(table, y)
   {
-    assert SimpleCanon(table, x) != SimpleCanon(table, y) by {
-      reveal SimpleCanon();
-      assert TerminalLocation([Map(x)]).canonicalPath(table) != TerminalLocation([Map(y)]).canonicalPath(table) by {
-        OnePart([Map(x)]);
-        OnePart([Map(y)]);
-        CanonicalPartMapUnique(Map(x), Map(y));
-        var prefix := UTF8.Encode(table).value + UInt64ToSeq(1 as uint64);
-        assert TerminalLocation([Map(x)]).canonicalPath(table) == prefix + CanonicalPart(Map(x));
-        assert TerminalLocation([Map(y)]).canonicalPath(table) == prefix + CanonicalPart(Map(y));
-        assert CanonicalPart(Map(x)) != CanonicalPart(Map(y));
-        OnePlusOne(prefix, CanonicalPart(Map(x)), CanonicalPart(Map(y)));
-        assert TerminalLocation([Map(x)]).canonicalPath(table) != TerminalLocation([Map(y)]).canonicalPath(table);
-      }
-    }
+    reveal SimpleCanon();
+    FullPathUnique(table);
   }
 
   // x != y ==> SimpleCanon(x) != SimpleCanon(y), so we can map with it
