DynamoDbEncryption/dafny/JsonEncryptor/src/JsonPath.dfy
@@ -1,0 +1,201 @@
+// Copyright Amazon.com Inc. or its affiliates. All Rights Reserved.
+// SPDX-License-Identifier: Apache-2.0
+
+include "AwsCryptographyDbEncryptionSdkDynamoDbJsonOperations.dfy"
+include "Util.dfy"
+
+module {:options "-functionSyntax:4"} JsonPathMod {
+  export
+    provides
+      Wrappers,
+      ValidPath,
+      PrettyString,
+      StandardString,
+      Parse
+    reveals
+      JsonPath,
+      JsonPathBase
+
+  import opened Wrappers
+  import opened StandardLibrary
+
+  datatype JsonPathBase = JsonPathBase (path : seq<string>)
+  type JsonPath = x : JsonPathBase | ValidPath(x.path) witness *
+
+  predicate NonEmpty(path : seq<string>)
+  {
+    forall x <- path :: 0 < |x|
+  }
+
+  predicate ValidPath(path : seq<string>)
+  {
+    && 0 < |path|
+    && NonEmpty(path)
+  }
+
+  predicate Alpha(ch : char)
+  {
+    || 'a' <= ch <= 'z'
+    || 'A' <= ch <= 'Z'
+  }
+
+  predicate AlphaNumeric(ch : char)
+  {
+    || '0' <= ch <= '9'
+    || Alpha(ch)
+  }
+
+
+  predicate IsPlain(member : string)
+  {
+    if |member| == 0 then
+      false
+    else if !Alpha(member[0]) then
+      false
+    else
+      forall k <- member :: AlphaNumeric(k)
+  }
+
+  function {:tailrecursion} StandardString4(path : string) : string
+  {
+    if |path| == 0 then
+      ""
+    else if path[0] == '\'' then
+      "\\\'" + StandardString4(path[1..])
+    else if path[0] == '\\' then
+      "\\\\" + StandardString4(path[1..])
+    else
+      [path[0]] + StandardString4(path[1..])
+  }
+
+  function StandardString3(path : string) : string
+  {
+    "['" + StandardString4(path) + "']"
+  }
+
+  function PrettyString3(path : string) : string
+  {
+    if IsPlain(path) then
+      path
+    else
+      StandardString3(path)
+  }
+
+  function {:tailrecursion} PrettyString2(path : seq<string>) : string
+  {
+    if |path| == 0 then
+      ""
+    else
+      "." + PrettyString3(path[0]) + PrettyString2(path[1..])
+  }
+
+  function {:tailrecursion} StandardString2(path : seq<string>) : string
+  {
+    if |path| == 0 then
+      ""
+    else
+      "." + StandardString3(path[0]) + StandardString2(path[1..])
+  }
+
+  function PrettyString(path : JsonPath) : string
+  {
+    if |path.path| == 0 then
+      ""
+    else if |path.path| == 1 && IsPlain(path.path[0]) then
+      path.path[0]
+    else
+      "$" + PrettyString2(path.path)
+  }
+
+  function StandardString(path : JsonPath) : string
+  {
+    if |path.path| == 0 then
+      ""
+    else
+      "$" + StandardString2(path.path)
+  }
+
+  function {:tailrecursion} GetString(input : string, delim : char, acc : nat := 0, accStr : string := "", orig : string := input) : (ret : Result<(nat,string), string>)
+    requires |input| + acc == |orig|
+    ensures ret.Success? ==> ret.value.0 <= |orig|
+  {
+    if |input| == 0 then
+      Success((acc, accStr))
+    else if input[0] == delim then
+      Success((acc, accStr))
+    else if input[0] == '\\' then
+      if |input| == 1 then
+        Failure("Trailing backslash : " + orig)
+      else if input[1] == '\\' then
+        GetString(input[2..], delim, acc+2, accStr + "\\", orig)
+      else if input[1] == '"' then
+        GetString(input[2..], delim, acc+2, accStr + "\"", orig)
+      else if input[1] == '\'' then
+        GetString(input[2..], delim, acc+2, accStr + "'", orig)
+      else
+        Failure("Backslash must only be followed by another backslash or a quote : " + orig)
+    else
+      GetString(input[1..], delim, acc+1, accStr + [input[0]], orig)
+  }
+
+  // return (nextPart, theRest)
+  function Parse3(input : string, acc : seq<string> := []) : (ret : Result<(string, string), string>)
+    requires 1 < |input|
+    requires input[0] == '.'
+    ensures ret.Success? ==>
+              && 0 < |ret.value.0|
+              && |ret.value.1| < |input|
+  {
+    if input[1] == '[' then
+      if |input| == 2 then
+        Failure("Malformed JSONPath segment : .[")
+      else if input[2] != '\'' && input[2] != '"' then
+        Failure("Malformed JSONPath segment started '.[' but not followed by a quote : " + input)
+      else if |input| == 3 then
+        Failure("Malformed JSONPath segment : " + input)
+      else
+        var (len,val) :- GetString(input[3..], input[2]);
+        :- Need(0 < |val|, "Bad1");
+        :- Need(4+len < |input|, "Bad2");
+        :- Need(input[3+len] == input[2], "No close quote");
+        :- Need(input[4+len] == ']', "Bad3");
+        Success((val, input[5+len..]))
+    else
+      var (len,val) :- GetString(input[1..], '.');
+      :- Need(0 < |val|, "Bad4");
+      Success((val, input[1+len..]))
+
+  }
+
+  function {:tailrecursion} Parse2(input : string, acc : seq<string> := []) : (ret : Result<seq<string>, string>)
+    requires NonEmpty(acc)
+    requires 0 < |input| || 0 < |acc|
+    ensures ret.Success? ==> ValidPath(ret.value)
+    decreases |input|
+  {
+    if |input| == 0 then
+      Success(acc)
+    else if input[0] != '.' then
+      Failure("JSONPath segment did not start with '.'")
+    else if |input| == 1 then
+      Failure("JSONPath segment was just a '.'")
+    else
+      var parts :- Parse3(input);
+      Parse2(parts.1, acc + [parts.0])
+  }
+
+  function Parse(input : string) : Result<JsonPath, string>
+  {
+    if |input| == 0 then
+      Failure("JSONPath cannot be an empty string.")
+    else if input[0] == '$' then
+      :- Need(1 < |input| && input[1] == '.', "JSONPath must start '$.'");
+      var parts :- Parse2(input[1..]);
+      Success(JsonPathBase(path := parts))
+    else if IsPlain(input) then
+      Success(JsonPathBase(path := [input]))
+    else
+      Failure("JSONPath '" + input + "' did not start with a '$', and yet contained special characters.")
+
+  }
+}
