DynamoDbEncryption/dafny/JsonEncryptor/test/JsonPath.dfy
@@ -1,0 +1,40 @@
+// Copyright Amazon.com Inc. or its affiliates. All Rights Reserved.
+// SPDX-License-Identifier: Apache-2.0
+include "../src/JsonPath.dfy"
+
+module JsonPathTest {
+  import opened JsonPathMod
+
+    method {:test} TestRoundTrips() {
+      var jp :- expect Parse("$.a.b.c");
+      expect jp == JsonPathBase(path := ["a", "b", "c"]);
+      expect PrettyString(jp) == "$.a.b.c";
+      expect StandardString(jp) == "$.['a'].['b'].['c']";
+
+      jp :- expect Parse("$.['a'].['bb'].['ccc']");
+      expect jp == JsonPathBase(path := ["a", "bb", "ccc"]);
+      print "\n", PrettyString(jp), "\n";
+      print "\n", StandardString(jp), "\n";
+      expect PrettyString(jp) == "$.a.bb.ccc";
+      expect StandardString(jp) == "$.['a'].['bb'].['ccc']";
+
+      jp :- expect Parse("abc");
+      expect jp == JsonPathBase(path := ["abc"]);
+      expect PrettyString(jp) == "abc";
+      expect StandardString(jp) == "$.['abc']";
+
+      jp :- expect Parse("$.[\"'\"].['bb'].[\"ccc\"]");
+      expect jp == JsonPathBase(path := ["'", "bb", "ccc"]);
+      expect PrettyString(jp) == "$.['\\\''].bb.ccc";
+      expect StandardString(jp) == "$.['\\\''].['bb'].['ccc']";
+
+      jp :- expect Parse("$.['a'].['b\\\\b'].['\\\'\\\\\\\''].[\"\\\"\"]");
+      expect jp == JsonPathBase(path := ["a", "b\\b", "'\\'", "\""]);
+      print "\n", PrettyString(jp), "\n";
+      print "\n", StandardString(jp), "\n";
+      expect PrettyString(jp) == "$.a.['b\\\\b'].['\\\'\\\\\\\''].['\"']";
+      expect StandardString(jp) == "$.['a'].['b\\\\b'].['\\\'\\\\\\\''].['\"']";
+
+    }
+
+}
