DynamoDbEncryption/dafny/JsonEncryptor/Model/JsonEncryptor.smithy
@@ -2,30 +2,27 @@
 // SPDX-License-Identifier: Apache-2.0
 namespace aws.cryptography.dbEncryptionSdk.dynamoDb.json
 
-use aws.polymorph#localService
-use aws.polymorph#javadoc
-use aws.polymorph#dafnyUtf8Bytes
-
-use aws.cryptography.materialProviders#KeyringReference
+use aws.cryptography.dbEncryptionSdk.structuredEncryption#CryptoAction
+use aws.cryptography.dbEncryptionSdk.structuredEncryption#StructuredEncryption
+use aws.cryptography.materialProviders#AwsCryptographicMaterialProviders
 use aws.cryptography.materialProviders#CryptographicMaterialsManagerReference
 use aws.cryptography.materialProviders#DBEAlgorithmSuiteId
 use aws.cryptography.materialProviders#EncryptedDataKeyList
 use aws.cryptography.materialProviders#EncryptionContext
-// use aws.cryptography.encryptionSdk#FrameLength
-
-use aws.cryptography.materialProviders#AwsCryptographicMaterialProviders
+use aws.cryptography.materialProviders#KeyringReference
 use aws.cryptography.primitives#AwsCryptographicPrimitives
-use aws.cryptography.dbEncryptionSdk.structuredEncryption#StructuredEncryption
-use aws.cryptography.dbEncryptionSdk.structuredEncryption#CryptoAction
+use aws.polymorph#dafnyUtf8Bytes
+use aws.polymorph#javadoc
+use aws.polymorph#localService
 
 @localService(
-  sdkId: "JsonEncryptor",
-  config: JsonEncryptorConfig,
-  dependencies: [
-    AwsCryptographicPrimitives,
-    AwsCryptographicMaterialProviders,
-    StructuredEncryption,
-  ]
+    sdkId: "JsonEncryptor",
+    config: JsonEncryptorConfig,
+    dependencies: [
+        AwsCryptographicPrimitives,
+        AwsCryptographicMaterialProviders,
+        StructuredEncryption
+    ]
 )
 service JsonEncryptor {
     version: "2024-02-14",
@@ -38,39 +35,63 @@ string Utf8Bytes
 
 // list of member names, JSONPath format
 list MemberNameList {
-  member: String
+    member: String
 }
+
+@enum([
+  {
+    name: "FORCE_PLAINTEXT_WRITE_ALLOW_PLAINTEXT_READ",
+    value: "FORCE_PLAINTEXT_WRITE_ALLOW_PLAINTEXT_READ",
+  },
+  {
+    name: "FORBID_PLAINTEXT_WRITE_ALLOW_PLAINTEXT_READ",
+    value: "FORBID_PLAINTEXT_WRITE_ALLOW_PLAINTEXT_READ",
+  },
+  {
+    name: "FORBID_PLAINTEXT_WRITE_FORBID_PLAINTEXT_READ",
+    value: "FORBID_PLAINTEXT_WRITE_FORBID_PLAINTEXT_READ",
+  },
+])
+string PlaintextOverride
 
 // Json structure. One day, we should add `Document` to allow language's JSON format
 union Json {
-  utf8 : Utf8Bytes,
-  text : String
+    utf8: Utf8Bytes,
+    text: String
 }
 
 // Associate a CryptoAction with a member name
 map MemberActions {
     key: String,
-    value: Action,
+    value: CryptoAction
 }
 
-union Action {
-  crypto : CryptoAction,
-  dbesdk : JsonEncrypt
+// if A.B is in MemberEncrypt,
+// then we collect all the A.B.* from MemberActions and DecoyMap and make a separate config.
+// encrypt the object then replace all the A.B.* with "A.B => SIGN_ONLY"
+map MemberEncrypt {
+    key: String,
+    value: JsonEncrypt
+}
+
+// if A.B in DecoyMap then encrypted object has "A.B" : value
+// and encrypted bytes are in A.aws_dbe_a_B
+map DecoyMap {
+    key: String,
+    // must refer to something that is ENCRYPT_AND_SIGN
+    value: String// Should this be `Json`?
 }
 
 structure JsonEncrypt {
-
-  // Requires a Keyring XOR a CMM
-  @javadoc("The Keyring that should be used to wrap and unwrap data keys. If specified a Default Cryptographic Materials Manager with this Keyring is used to obtain materials for encryption and decryption. Either a Keyring or a Cryptographic Materials Manager must be specified.")
-  keyring: KeyringReference,
-  @javadoc("The Cryptographic Materials Manager that is used to obtain materials for encryption and decryption.  Either a Keyring or a Cryptographic Materials Manager must be specified.")
-  cmm: CryptographicMaterialsManagerReference,
-
-  @javadoc("An ID for the algorithm suite to use during encryption and decryption.")
-  algorithmSuiteId: DBEAlgorithmSuiteId,
-
-  @javadoc("Extra key-value pairs to include in the required encryption context.")
-  encryptionContext: aws.cryptography.materialProviders#EncryptionContext,
+    // Requires a Keyring XOR a CMM
+    @javadoc("The Keyring that should be used to wrap and unwrap data keys. If specified a Default Cryptographic Materials Manager with this Keyring is used to obtain materials for encryption and decryption. Either a Keyring or a Cryptographic Materials Manager must be specified.")
+    keyring: KeyringReference,
+    @javadoc("The Cryptographic Materials Manager that is used to obtain materials for encryption and decryption.  Either a Keyring or a Cryptographic Materials Manager must be specified.")
+    cmm: CryptographicMaterialsManagerReference,
+    @javadoc("An ID for the algorithm suite to use during encryption and decryption.")
+    algorithmSuiteId: DBEAlgorithmSuiteId,
+    @javadoc("Extra key-value pairs to include in the required encryption context.")
+    encryptionContext: aws.cryptography.materialProviders#EncryptionContext
 }
 
 @javadoc("The configuration for the client-side encryption of JSON objects.")
@@ -92,6 +113,15 @@ structure JsonEncryptorConfig {
     @required
     @javadoc("Setting for encryption and decryption.")
     encrypt: JsonEncrypt,
+
+    @javadoc("Encrypt this part separately, with different materials.")
+    nestedEncryption: MemberEncrypt,
+
+    @javadoc("These members are replaced by the decoy value, encrypted bytes hidden elsewhere. Member must be same type as decoy value.")
+    decoys: DecoyMap,
+
+    @javadoc("A configuration that overrides encryption and/or decryption to instead pass through and write and/or read plaintext. Used to update plaintext processes to fully use client-side encryption.")
+    plaintextOverride: PlaintextOverride
 }
 
 @javadoc("A parsed version of the header that was written with or read on an encrypted Json object.")
@@ -99,15 +129,19 @@ structure ParsedHeader {
     @required
     @javadoc("The non-DO_NOTHING Crypto Actions that were configured when this object was originally encrypted.")
     memberActionsOnEncrypt: MemberActions,
+
     @required
     @javadoc("The ID of the algorithm suite that was used to encrypt this object.")
     algorithmSuiteId: DBEAlgorithmSuiteId,
+
     @required
     @javadoc("The encrypted data keys that are stored in the header of this object.")
     encryptedDataKeys: EncryptedDataKeyList,
+
     @required
     @javadoc("The portion of the encryption context that was stored in the header of this object.")
     storedEncryptionContext: EncryptionContext,
+
     @required
     @javadoc("The full encryption context.")
     encryptionContext: EncryptionContext
@@ -116,20 +150,20 @@ structure ParsedHeader {
 @javadoc("Encrypt a Json object.")
 operation EncryptObject {
     input: EncryptObjectInput,
-    output: EncryptObjectOutput,
+    output: EncryptObjectOutput
 }
 
 @javadoc("Decrypt a Json object.")
 operation DecryptObject {
     input: DecryptObjectInput,
-    output: DecryptObjectOutput,
+    output: DecryptObjectOutput
 }
 
 @javadoc("Inputs for encrypting a JSON object.")
 structure EncryptObjectInput {
     @required
     @javadoc("The JSON object to encrypt.")
-    plaintextObject: Json,
+    plaintextObject: Json
 }
 
 @javadoc("Outputs for encrypting a JSON object.")
@@ -137,16 +171,15 @@ structure EncryptObjectOutput {
     @required
     @javadoc("The encrypted JSON object.")
     encryptedObject: Json,
-
     @javadoc("A parsed version of the header written with the encrypted JSON object.")
-    parsedHeader: ParsedHeader,
+    parsedHeader: ParsedHeader
 }
 
 @javadoc("Inputs for decrypting a JSON object.")
 structure DecryptObjectInput {
     @required
     @javadoc("The encrypted JSON object to decrypt.")
-    encryptedObject: Json,
+    encryptedObject: Json
 }
 
 @javadoc("Outputs for decrypting a JSON object.")
@@ -154,21 +187,22 @@ structure DecryptObjectOutput {
     @required
     @javadoc("The decrypted JSON object.")
     plaintextObject: Json,
-
     @javadoc("A parsed version of the header on the encrypted JSON object.")
-    parsedHeader: ParsedHeader,
+    parsedHeader: ParsedHeader
 }
 
 @aws.polymorph#reference(service: aws.cryptography.primitives#AwsCryptographicPrimitives)
 structure AtomicPrimitivesReference {}
-@aws.polymorph#reference(service: aws.cryptography.dbEncryptionSdk.structuredEncryption#StructuredEncryption)
+
+@aws.polymorph#reference(
+    service: aws.cryptography.dbEncryptionSdk.structuredEncryption#StructuredEncryption
+)
 structure StructuredEncryptionReference {}
 
-/////////////
+/// //////////
 // Errors
-
 @error("client")
 structure JsonEncryptorException {
-  @required
-  message: String,
+    @required
+    message: String
 }
