Makefile
@@ -1,3 +1,49 @@
+# Copyright Amazon.com Inc. or its affiliates. All Rights Reserved.
+# SPDX-License-Identifier: Apache-2.0
+
+# This finds all Dafny projects in this repository
+# This makes building root level targets for each project easy
+PROJECTS = $(shell  find . -mindepth 2 -maxdepth 2 -type f -name "Makefile" | xargs dirname | xargs basename)
+
+verify:
+	$(foreach PROJECT, $(PROJECTS), \
+		$(MAKE) -C $(PROJECT) verify CORES=4 && \
+	) true
+
+dafny-reportgenerator:
+	$(foreach PROJECT, $(PROJECTS), \
+		$(MAKE) -C $(PROJECT) dafny-reportgenerator && \
+	) true
+
+clean-dafny-report:
+	$(foreach PROJECT, $(PROJECTS), \
+		$(MAKE) -C $(PROJECT) clean-dafny-report && \
+	) true
+
+format_dafny:
+	$(foreach PROJECT, $(PROJECTS), \
+		$(MAKE) -C $(PROJECT) format_dafny && \
+	) true
+
+format_net:
+	$(foreach PROJECT, $(PROJECTS), \
+		$(MAKE) -C $(PROJECT) format_net && \
+	) true
+
+format_java_misc:
+	npx prettier --plugin=prettier-plugin-java . --write
+
+format_java_misc-check:
+	npx prettier --plugin=prettier-plugin-java . --check
+
+setup_prettier:
+	npm i --no-save prettier prettier-plugin-java
+
+polymorph_code_gen:
+	$(foreach PROJECT, $(PROJECTS), \
+		$(MAKE) -C $(PROJECT) polymorph_code_gen && \
+	) true
+
 duvet: | duvet_extract duvet_report
 
 duvet_extract:
@@ -11,4 +57,5 @@ duvet_report:
 		--source-pattern "DynamoDbEncryption/dafny/**/*.dfy" \
 		--source-pattern "DynamoDbEncryption/dafny/**/*.smithy" \
 		--source-pattern "DynamoDbEncryption/runtimes/java/src/main/java/**/*.java" \
+		--source-pattern "(# //=,# //#).github/workflows/duvet.yaml" \
 		--html specification_compliance_report.html
